\section{Proofs of auxiliary results}
{\colrbf need modification}
\begin{proof}[Proof of Proposition~\ref{prop:Thm1ProofProp2}]
In its reparametrized version, (\ref{eqn:EstEqn2}) becomes
%
\begin{align}
\widehat \bfT_j = \argmin_{\bfT_j} \left\{ \frac{1}{n} \sum_{k=1}^K \| (\bfY^k - \bfX^k \widehat \bfB^k) \bfT_j^k \|^2 + \gamma_n \sum_{j \neq j', g \in \cG_y^{jj'}} \| \bfT_{jj'}^{[g]} \| \right\}
\end{align}
%
with $\bfT_{jj'}^{[g]} := (T_{jj'}^k)_{k \in g}$. Now for any $\bfT_j \in \BM(q, K)$ we have
%
$$
\frac{1}{n} \sum_{k=1}^K \| (\bfY^k - \bfX^k \widehat \bfB^k) \widehat \bfT_j^k \|^2 + \gamma_n \sum_{j \neq j', g \in \cG_y^{jj'}} \| \widehat \bfT_{jj'}^{[g]} \| \leq
\frac{1}{n} \sum_{k=1}^K \| (\bfY^k - \bfX^k \widehat \bfB^k) \bfT_j^k \|^2 + \gamma_n \sum_{j \neq j', g \in \cG_y^{jj'}} \| \bfT_{jj'}^{[g]} \|
$$
%
For $\bfT_j = \bfT_{0,j}$ this reduces to
%
\begin{align}\label{eqn::Thm1ProofProp2Eqn1}
\sum_{k=1}^K (\bfd_j^k)^T \widehat \bfS^k \bfd_j^k & \leq - 2 \sum_{k=1}^K (\bfd_j^k)^T \widehat \bfS^k \bfT_{0,j}^k + \gamma_n \sum_{j \neq j', g \in \cG_y^{jj'}} \left( \| \bfT_{jj'}^{[g]} \| -  \| \bfT_{jj'}^{[g]} + \bfd_{jj'}^{[g]}\| \right)
\end{align}
%
with $\bfd_{j}^k := \widehat \bfT_j^k - \bfT_{0,j}^k$ etc. For the $k^\text{th}$ summand in the first term on the right hand side, since $d_{jj}^k = 0$, $\widehat \bfE^k \bfd_j^k = \widehat \bfE_{-j}^k \bfd_{-j}^k$. Thus
%
\begin{align*}
\sum_{k=1}^K \left| (\bfd_j^k)^T \widehat \bfS^k \bfT_{0,j}^k \right| &=
\sum_{k=1}^K \left| \bfd_j^k. \frac{1}{n} (\widehat \bfE^k)^T \widehat \bfE^k \bfT_{0,j}^k \right| \\
& \leq \sum_{k=1}^K \left\| \frac{1}{n} (\widehat \bfE_{-j}^k)^T \widehat \bfE^k \bfT_{0,j}^k \right\|_\infty \| \bfd_{-j}^k \|_1 \\
& \leq \BQ_0 \sqrt {| g_{\max}|} \sum_{j \neq j', g \in \cG_y^{jj'}} \| \bfd_{jj'}^{[g]} \|
\end{align*}
%
by assumption (T2). For the second term, suppose $\cS_{0,j}$ is the support of $\Theta_{0,j}$, i.e. $\cS_{0,j} = \{ (j',g): \bftheta_{jj'}^{[g]} \neq 0 \}$. Then
%
\begin{align*}
\sum_{j \neq j', g \in \cG_y^{jj'}} \left( \| \bfT_{jj'}^{[g]} \| -  \| \bfT_{jj'}^{[g]} + \bfd_{jj'}^{[g]}\| \right) & \leq
\sum_{(j',g) \in \cS_{0,j}} \left( \| \bfT_{jj'}^{[g]} \| -  \| \bfT_{jj'}^{[g]} + \bfd_{jj'}^{[g]}\| \right) -
\sum_{(j',g) \notin \cS_{0,j}} \| \bfd_{jj'}^{[g]} \|\\
& \leq \sum_{(j',g) \in \cS_{0,j}} \| \bfd_{jj'}^{[g]} \| - \sum_{(j',g) \notin \cS_{0,j}} \| \bfd_{jj'}^{[g]} \|
\end{align*}
%$ \| \bfT_{jj'}^{[g]} \| -  \| \bfT_{jj'}^{[g]} + \bfd_{jj'}^{[g]}\| \leq \| \bfd_{jj'}^{[g]}\|$ by triangle inequality, and then $ \| \bfd_{jj'}^{[g]}\| \leq \sum_{k \in g} | d_{jj'}^k | $, 
so that by choice of $\gamma_n$ (\ref{eqn::Thm1ProofProp2Eqn1}) reduces to
%
\begin{align}\label{eqn:Thm1ProofProp2Eqn3}
\sum_{k=1}^K (\bfd_j^k)^T \widehat \bfS^k \bfd_j^k & \leq 
\frac{\gamma_n}{2} \left[ \sum_{(j',g) \in \cS_{0,j}} \| \bfd_{jj'}^{[g]} \| + \sum_{(j',g) \notin \cS_{0,j}} \| \bfd_{jj'}^{[g]} \| \right] +
\gamma_n \left[ \sum_{(j',g) \in \cS_{0,j}} \| \bfd_{jj'}^{[g]} \| - \sum_{(j',g) \notin \cS_{0,j}} \| \bfd_{jj'}^{[g]} \| \right] \notag\\
& = \frac{3 \gamma_n}{2} \sum_{(j',g) \in \cS_{0,j}} \| \bfd_{jj'}^{[g]} \| - \frac{\gamma_n}{2} \sum_{(j',g) \notin \cS_{0,j}} \| \bfd_{jj'}^{[g]} \| \notag\\
& \leq \frac{3 \gamma_n}{2} \sum_{j \neq j', g \in \cG_y^{jj'}} \| \bfd_{jj'}^{[g]} \|
\end{align}
%
Since the left hand side is $\geq 0$, this also implies
%
$$
\sum_{(j',g) \notin \cS_{0,j}} \| \bfd_{jj'}^{[g]} \| \leq 3 \sum_{(j',g) \in \cS_{0,j}} \| \bfd_{jj'}^{[g]} \| \quad \Rightarrow
\sum_{j \neq j', g \in \cG_y^{jj'}} \| \bfd_{jj'}^{[g]} \| \leq
4 \sum_{(j',g) \in \cS_{0,j}} \| \bfd_{jj'}^{[g]} \| \leq 4 \sqrt{s_j} \| \bfD_j \|_F
$$
% 
with $\bfD_j = (\bfd_j^k)_{k \in \cI_K}$. Now the RE condition on $\widehat \bfS^k$ means that
%
$$
\sum_{k=1}^K (\bfd_j^k)^T \widehat \bfS^k \bfd_j^k \geq 
\sum_{k=1}^K \left( \psi_k \| \bfd_j^k \|^2 - \phi_k \| \bfd_j^k \|_1^2 \right) \geq
\psi \| \bfD_j \|_F^2 - \phi \| \bfD_j \|_1^2 \geq 
(\psi - Kq \phi ) \| \bfD_j \|_F^2 \geq \frac{\psi}{2}  \| \bfD_j \|_F^2
$$
%
by assumption (T3).

Thus we finally have
%
\begin{align}\label{eqn:Thm1ProofProp2Eqn2}
\frac{\psi}{3} \| \bfD_j \|_F^2 & \leq
\gamma_n \sum_{j \neq j', g \in \cG_y^{jj'}} \| \bfd_{jj'}^{[g]} \| \leq
4 \gamma_n \sqrt{s_j} \| \bfD_j\|_F
\end{align}
%
Since
%
$$
(\bfD_j)_{j',k} = \widehat T_{jj'}^k - T_{0,jj'}^k = \begin{cases}
0 \text{ if } j = j'\\
-(\widehat \theta_{jj'}^k - \theta_{0,jj'}^k ) \text{ if } j \neq j'
\end{cases}
$$
%
The bounds in (\ref{eqn:Thm1ProofProp2Bd1}) and (\ref{eqn:Thm1ProofProp2Bd2}) are obtained by replacing the corresponding elements in (\ref{eqn:Thm1ProofProp2Eqn2}).

For the bound on $| \widehat \cS_j|$, notice that if $\hat \bftheta_{jj'}^{[g]} \neq 0$ for some $(j',g)$,
%
\begin{align*}
\frac{1}{n} \sum_{k \in g} \left| ((\widehat \bfE_{-j}^k)^T \widehat \bfE^k ( \widehat \bfT_j^k - \bfT_{0,j}^k ))^{j'} \right| & \geq
\frac{1}{n} \sum_{k \in g} \left| ((\widehat \bfE_{-j}^k)^T \widehat \bfE^k \widehat \bfT_j^k )^{j'} \right| - \frac{1}{n} \sum_{k \in g} \left| ((\widehat \bfE_{-j}^k)^T \widehat \bfE^k \bfT_{0,j}^k )^{j'} \right|\\
& \geq |g| \gamma_n - \sum_{k \in g} \BQ ( v_\beta, \Sigma_x^k, \Sigma_y^k )
\end{align*}
%
using the KKT condition for (\ref{eqn:EstEqn2}) and assumption (T2). The choice of $\gamma_n$ now ensures that the right hand side is $\geq 3|g| \gamma_n / 4$. Hence
%
\begin{align*}
| \hat \cS_j| & \leq \sum_{(j',g) \in \widehat \cS_j} \frac{16}{9 n^2 |g|^2 \gamma_n^2 } \sum_{k \in g} \left| ((\widehat \bfE_{-j}^k)^T \widehat \bfE^k ( \widehat \bfT_j^k - \bfT_{0,j}^k ))^{j'} \right|^2\\
& \leq \frac{16}{9 \gamma_n^2} \sum_{k=1}^K \frac{1}{n} \left\| (\widehat \bfE_{-j}^k)^T \widehat \bfE^k ( \widehat \bfT_j^k - \bfT_{0,j}^k ) \right\|^2 \\
& = \frac{16}{9 \gamma_n^2} \sum_{k=1}^K (\bfd_j^k)^T \widehat \bfS^k \bfd_j^k \\
& \leq \frac{8}{3 \gamma_n} \sum_{j \neq j', g \in \cG_y^{jj'}} \| \bfd_{jj'}^{[g]} \| \leq \frac{128 s_j}{\psi} 
\end{align*}
%
using (\ref{eqn:Thm1ProofProp2Eqn3}) and (\ref{eqn:Thm1ProofProp2Eqn2}).
\end{proof}

\begin{proof}[Proof of Lemma~\ref{lemma:ErrorRElemma1}]
This is same as Lemma 2 in Appendix B of \cite{LinEtal16} and its proof can be found there.
\end{proof}

\begin{proof}[Proof of Lemma~\ref{lemma:ErrorRElemma2}]
This is a part of Lemma 3 of Appendix B in \cite{LinEtal16}, and is proved therein. 
\end{proof}

\begin{proof}[Proof of Lemma~\ref{Lemma:ThmTestingLemma}]
To show \eqref{eqn:ThmTestingProofeq3} we have
%
\begin{align*}
\frac{1}{\sqrt n \widehat s_i}  \widehat \Omega_y^{1/2} \bfE^T \bfR_i =
\frac{1}{\sqrt n \widehat s_i}  (\widehat \Omega_y^{1/2} - \Omega_y^{1/2}) \bfE^T \bfR_i +
\frac{1}{\sqrt n \widehat s_i}  \Omega_y^{1/2} \bfE^T \bfR_i
\end{align*}
%
The second summand is distributed as $\cN_q ({\bf 0}, \bfI)$. For the first summand,
%
\begin{align*}
\frac{1}{\sqrt n}  \left\| (\widehat \Omega_y^{1/2} - \Omega_y^{1/2}) \bfE^T \bfR_i \right\|_\infty & \leq
\frac{1}{\sqrt n}  \left\| \widehat \Omega_y^{1/2} - \Omega_y^{1/2} \right\|_\infty  \left\| \bfE^T \bfR_i \right\|_1 \\
& \leq \sqrt n v_\Omega \frac{1}{n} \left[ \| \bfE^T (\bfX_i -  \bfX_{-i} \bfzeta_i ) \|_1 + \| \bfE^T \bfX_{-i} (\widehat \bfzeta_i - \bfzeta_{0,i} ) \|_1 \right] \\
& \leq \sqrt n v_\Omega \frac{1}{n} \left[ \| \bfE^T \bfX_i \|_\infty + \| \bfE^T \bfX_{-i} \|_\infty
\left\{ \| \bfzeta_i  \|_1 + \| \widehat \bfzeta_i - \bfzeta_i  \|_1 \right\} \right] \notag\\
& \leq \sqrt n v_\Omega \left[ \frac{1}{n} \| \bfE^T \bfX_i \|_\infty + 
\frac{1 + v_\zeta}{n} \| \bfE^T \bfX_{-i} \|_\infty \right] \\
& \leq \sqrt n v_\Omega (2 + v_\zeta) .\frac{1}{n} \| \bfE^T \bfX \|_\infty
\end{align*}
%
because $\Omega_x$ is diagonally dominant implies $\| \bfzeta_i \|_1 = \sum_{i' \neq i} |\omega_{x,ii'}|/ \omega_{x,ii} \leq 1$, and using assumption (C1). Applying Lemma~\ref{lemma:ErrorRElemma2}, the following holds:
%
\begin{align}\label{eqn:ThmTestingProofeq31}
\frac{1}{\sqrt n}  \left\| (\widehat \Omega_y^{1/2} - \Omega_y^{1/2}) \bfE^T \bfR_i \right\|_\infty & \leq v_\Omega (2 + v_\zeta) c_2 [ \Lambda_{\max} (\Sigma_x) \Lambda_{\max} (\Sigma_e) ]^{1/2} \sqrt{ \log(pq)}
\end{align}
%
with probability $ \geq 1 - 6c_1 \exp [-(c_2^2-1) \log(pq)]$ for some $c_1 >0, c_2 > 1$.

On the other hand
%
\begin{align*}
s_i^2 := \frac{1}{n} \left\| \bfX_i - \bfX_{-i}  \bfzeta_i \right\|^2 & \leq 
\widehat s_i^2 + \frac{1}{n} \left\| \bfX_{-i} (\widehat \bfzeta_i - \bfzeta_{0,i} ) \right\|^2
\leq \widehat s_i^2 + \| \widehat \bfzeta_i - \bfzeta_{0,i} \|_1^2 \left\| \frac{1}{n} \bfX_{-i}^T \bfX_{-i} \right\|_\infty
\end{align*}
%
which implies $s_i \leq \widehat s_i + v_\zeta \sqrt{ V_x}$. By applying Lemma 8 of \cite{RavikumarEtal11},
%
\begin{align}\label{eqn:ThmTestingProofeq32}
\left\| \frac{1}{n} \bfX_{-i}^T \bfX_{-i} \right\|_\infty \leq
\left\| \frac{1}{n} \bfX^T \bfX \right\|_\infty \leq V_x
\end{align}
%
with probability $ \geq 1 - 1/p^{\tau_1-2}, \tau_1>2$, and
%
\begin{align}\label{eqn:ThmTestingProofeq33}
n \geq 512 ( 1 + 4 \Lambda_{\max} (\Sigma_{x}))^4 \max_i (\sigma_{x,ii} )^4 \log (4p^{\tau_1})
\end{align}
%
On the other hand, by Chebyshev inequality, for any $\epsilon>0$
%
$$
P\left( | s_i - \sigma_{x,i,-i}| \geq \epsilon \right) \leq \frac{\BV s_i}{\epsilon^2} =
\frac{\kappa_i}{n \epsilon^2}
$$
%
Taking $\epsilon = n^{-1/4}$, we have $s_i \geq \sigma_{x,i,-i} - n^{-1/4}$ with probability $\geq 1 - \kappa_i n^{-1/2}$. Then, for $n$ satisfying \eqref{eqn:ThmTestingProofeq32} and $\sigma_{x,i,-i} - n^{-1/4} >  v_\zeta \sqrt{ V_x}$, we get the bound with the above probability:
%
\begin{align}\label{eqn:ThmTestingProofeq34}
\frac{1}{\widehat s_i} \leq \frac{1}{\sigma_{x,i,-i} - n^{-1/4} - v_\zeta \sqrt{ V_x}}
\end{align}
%
Combining \eqref{eqn:ThmTestingProofeq31} and \eqref{eqn:ThmTestingProofeq34} gives the upper bound for the right hand side of \eqref{eqn:ThmTestingProofeq3} with the requisite probability and sample size conditions.

To prove \eqref{eqn:ThmTestingProofeq4} we have
%
\begin{align}\label{eqn:ThmTestingProofeq41}
\frac{1}{n} \| \bfR_i^T \bfX_{-i} \|_\infty & \leq
\frac{1}{n} \| (\bfX_i - \bfX_{-i} \bfzeta_{0,i})^T \bfX_{-i} \|_\infty +
\frac{1}{n} \| \bfX_{-i}^T \bfX_{-i} ( \widehat \bfzeta_i - \bfzeta_{0,i}) \|_\infty
\end{align}
%
Applying Lemma~\ref{lemma:ErrorRElemma2}, for $n \succsim \log(p-1)$ we have
%
%
\begin{align}
\frac{1}{n} \| (\bfX_i -  \bfX_{-i} \bfzeta_i )^T \bfX_{-i} \|_\infty \leq 
c_{7} [ \sigma_{x,i,-i} \Lambda_{\max} (\Sigma_{x, -i}) ]^{1/2} \sqrt{\frac{ \log (p-1)}{n}}
\end{align}
%
with probability $\geq 1 - 6c_{6} \exp [-(c_{7}^2-1) \log (p-1)]$ for some $c_{6} >0, c_{7} > 1$. By \eqref{eqn:ThmTestingProofeq32}, the second term on the right side of \eqref{eqn:ThmTestingProofeq41} is bounded above by $v_\zeta V_x$ with probability $ \geq 1 - 1/p^{\tau_1-2}$ and $n$ satisfying \eqref{eqn:ThmTestingProofeq33}. The bound of \eqref{eqn:ThmTestingProofeq4} now follows by conditions (C2), (C3) and \eqref{eqn:ThmTestingProofeq34}.
\end{proof}